OrderSig.v
@@ -1,3 +1,29 @@
+Set Implicit Arguments.
+
+Class ORDER A := Order {
+
+  LEQ : A -> A -> bool; 
+
+  leqRefl: forall x, true = LEQ x x;
+
+  leqTransTrue : forall x y z,
+      true = LEQ x y ->
+      true = LEQ y z ->
+      true = LEQ x z;
+
+  leqTransFalse : forall x y z,
+      false = LEQ x y ->
+      false = LEQ y z ->
+      false = LEQ x z;
+
+  leqSymm : forall x y,
+      false = LEQ x y ->
+      true = LEQ y x
+}.
+
+Extract Inductive bool => "Prelude.Bool" ["Prelude.True" "Prelude.False"].
+
+(*
 Module Type Order.
 
   Parameter (A:Type).
@@ -23,3 +49,27 @@ Module Type Order.
       true = LEQ y x).
 
 End Order.
+*)
+
+(*
+Record ORDER A := order {
+
+  LEQ : A -> A -> bool; 
+
+  leqRefl: forall x, true = LEQ x x;
+
+  leqTransTrue : forall x y z,
+      true = LEQ x y ->
+      true = LEQ y z ->
+      true = LEQ x z;
+
+  leqTransFalse : forall x y z,
+      false = LEQ x y ->
+      false = LEQ y z ->
+      false = LEQ x z;
+
+  leqSymm : forall x y,
+      false = LEQ x y ->
+      true = LEQ y x
+}.
+*)
