PQSig.v
@@ -1,7 +1,124 @@
 Set Implicit Arguments.
 
 Require Export OrderSig.
+Require Export List.
 
+Class MINQ {A PQ} `{ORDER A} := Minq {
+
+(*  O :> ORDER A; *)
+
+  empty:PQ;
+
+  insert: A -> PQ -> PQ;
+  findMin : PQ -> option A;
+  extractMin : PQ -> option (A*PQ);
+  toList : PQ -> list A;
+  meld : PQ -> PQ -> PQ
+}.
+
+Extract Inductive list => "[]" ["[]" "(:)"].
+Extract Inductive prod => "(,)" ["(,)"].
+Extract Inductive option => 
+  "Prelude.Maybe" ["Prelude.Just" "Prelude.Nothing"].
+
+Record DERP {A} `{ORDER A} (der:A -> A -> bool) := Derp {
+
+  derLeft : 
+    forall x y, 
+      true = der x y -> 
+      forall z, LEQ x z = LEQ y z;
+
+  derRight : 
+    forall x y, 
+      true = der x y -> 
+      forall z, LEQ z x = LEQ z y;
+
+  derRefl : forall x, der x x = true;
+
+  derSymm : forall x y, der x y = der y x;
+
+  derTrans : 
+    forall x y z, 
+      true = der x y ->
+      true = der y z ->
+      true = der x z
+}.
+
+Definition DER {A} `{ORDER A} := {der | DERP der}.
+
+
+Program Definition check {A} `{ORDER A} (s:DER) x y := s x y.
+
+
+Program Fixpoint listCount {A} `{ORDER A} (s:DER) x xs :=
+  match xs with
+    | nil => 0
+    | y::ys =>
+      let rest := listCount s x ys in
+        if s x y
+          then S rest
+          else rest
+  end.
+
+Class MINQV {A PQ} `{ORDER A} (m:MINQ) := Minqv {
+
+  count : DER -> A -> PQ -> nat;
+
+  toListCount :
+    forall s x y,
+      count s x y
+      = listCount s x (toList y);
+
+  countSAME :
+    forall s x y,
+      check s x y = true ->
+      forall inp, count s x inp = count s y inp;
+
+  emptyCount :
+    forall same x, count same x empty = 0;
+
+  insertCount :
+    forall same x inp y,
+      count same x (insert y inp) =
+      let oldCount := count same x inp in
+        if check same x y 
+          then S oldCount
+          else oldCount;
+
+  findMinCount :
+    forall inp,
+      match findMin inp with
+        | None => forall same x, count same x inp = 0
+        | Some x =>
+          forall same y, 
+            if check same y x
+              then count same y inp > 0
+              else count same y inp > 0 ->
+                LEQ x y = true
+      end;
+
+  extractMinCount :
+    forall inp,
+      match findMin inp with
+        | None => None = extractMin inp
+        | Some x => exists z,
+          Some (x,z) = extractMin inp
+          /\ forall same y,
+            let newCount := count same y z in
+              count same y inp =
+              if check same y x
+                then S newCount
+                else newCount
+      end;
+
+  meldCount :
+    forall same inp inq x,
+      count same x (meld inp inq) 
+      = count same x inp
+      + count same x inq
+}.
+  
+(*
 Module Type PQSig.
 
   Declare Module O:Order.
@@ -20,6 +137,7 @@ Module Type PQSig.
 
 End PQSig.
 
+(*
 Definition DERP a (leq:a -> a -> bool) (der:a -> a -> bool) := 
   (forall x y, true = der x y -> 
     ((forall z, leq x z = leq y z)
@@ -33,6 +151,7 @@ Definition DERP a (leq:a -> a -> bool) (der:a -> a -> bool) :=
     true = der x z).
 
 Definition DER a leq := {der | @DERP a leq der}.
+*)
 
 Module Type PQVerify.
 
@@ -106,3 +225,4 @@ Module Type PQVerify.
                                   + count same x inq.
 
 End PQVerify.
+*)
